proof/security/FO_UU.ec
@@ -951,7 +951,7 @@ rcondf{1} 30; 1: by auto => />;smt().
 swap{1} 11 -10 (* k1 *) ;swap {1} 29 -27 (* k0 *). (* fixme add swap for var names *)
 swap{2} [11..12] -10. (* k1 k2 *)
 seq 2 2 : (={glob A,k1} /\ k0{1} = k2{2}); 1: by auto.
-seq 32 19 : (={glob A,k1,pk,b,cm,CCA.sk,CCA.cstar, H2.invert, H2.mtgt, H1.bad, H2.merr, 
+ seq 32 19 : (={glob A,k1,pk,b,cm,CCA.sk,CCA.cstar, H2.invert, H2.mtgt, H1.bad, H2.merr, 
   H2.invert, RO1E.FunRO.f} /\ 
   !H2.invert{2} /\ 
   k0{1} = k2{2} /\  
@@ -962,8 +962,9 @@ seq 32 19 : (={glob A,k1,pk,b,cm,CCA.sk,CCA.cstar, H2.invert, H2.mtgt, H1.bad, H
   (forall c, Some c <> CCA.cstar{2} => assoc UU2.lD{1} c = assoc UU2.lD{2} c) /\
   (forall m, m <> H2.mtgt{2} => RO2.RO.m{1}.[m] = RO2.RO.m{2}.[m]) /\
   (!H1.bad{2} <=> 
-             Some H2.mtgt{2} = dec  CCA.sk{2}.`1.`2 (oget CCA.cstar{2})));
-    1: by auto => />; smt(mem_empty get_setE fdom_set @SmtMap @FSet @List).
+             Some H2.mtgt{2} = dec  CCA.sk{2}.`1.`2 (oget CCA.cstar{2}))).
+  auto => /> &2 f Hf kpair Hkpair b Hb m Hm.
+  smt(mem_empty get_setE fdom_set @SmtMap @FSet @List).
 
 case (H1.bad{1}).
 rnd;wp;call(:H1.bad,false,CCA.cstar{2} <> None /\ 
@@ -1180,9 +1181,15 @@ proc.
     + by islossless.
   + case (H1.bad). 
     + conseq(:nobias); 1: smt().
-      by rnd;rnd;auto => /> *;rewrite DBool.dbool_ll /=;smt(DBool.dbool1E).
+      rnd;rnd;auto => /> &hr ?; rewrite DBool.dbool_ll /=.
+       rewrite -(mu_eq _ (pred1 true)).
+       by move=> x; rewrite /pred1 /#.
+      by apply DBool.dbool1E.
     conseq(: b' = b); 1:smt(). 
-    by rnd;rnd;auto => /> *;rewrite DBool.dbool_ll /=;smt(DBool.dbool1E).
+    rnd;rnd;auto => /> &hr ?; rewrite DBool.dbool_ll /=.
+     rewrite -(mu_eq _ (pred1 b'{hr})).
+     by move=> x; rewrite /pred1 /= (eq_sym x).
+    by apply DBool.dbool1E.
   + by hoare; trivial.
 by done.
 qed.
